x86/MemoryC2.v
@@ -3,15 +3,195 @@ Require Import ASTC Integers Floats Values MemoryC Events Globalenvs Smallstep.
 Require Import Locations Stacklayout Conventions Linking.
 (** newly added **)
 Require Export Asm.
-Require Import Simulation Memory ValuesC.
+Require Import Simulation Memory ValuesC MemoryC.
 Require Import Skeleton ModSem Mod sflib AsmC Sem Syntax LinkingC Program SemProps.
 Require Import Lia.
 
 Set Implicit Arguments.
 
+
+Local Notation "a # b" := (PMap.get b a) (at level 1).
+Local Ltac simp := repeat (bsimpl; des; des_sumbool; ss; clarify).
+
+
 Local Opaque Z.mul.
 
 Existing Instance Val.mi_final.
+
+Inductive inj_range_block_wf (j: meminj) (m: mem) blk_src
+          (P: Z -> Prop) : Prop :=
+| inj_range_wf_empty
+    (REACH: j blk_src = None)
+    (BOT: P <1= bot1)
+| inj_range_wf_intro
+    blk_tgt delta
+    (DELTA: j blk_src = Some (blk_tgt, delta))
+    (ALIGN: forall chunk ofs k p, (range ofs (ofs + size_chunk chunk) <1= ((fun ofs => Mem.perm m blk_src ofs k p) \1/ P)) -> (align_chunk chunk | delta))
+    (RANGE: forall ofs,
+        (P (Ptrofs.unsigned ofs) \/
+         P (Ptrofs.unsigned ofs - 1) ->
+         delta >= 0 /\ 0 <= Ptrofs.unsigned ofs + delta <= Ptrofs.max_unsigned))
+.
+
+Definition inj_range_wf (j: meminj) (m: mem) (P: Values.block -> Z -> Prop) :=
+  forall blk, inj_range_block_wf j m blk (P blk).
+
+Lemma inj_range_wf_le j m P0 P1
+      (INJWF: inj_range_wf j m P0)
+      (PLE: P1 <2= P0)
+  :
+    inj_range_wf j m P1.
+Proof.
+  ii. destruct (INJWF blk).
+  - econs 1; eauto.
+  - econs 2; eauto; ii.
+    + eapply ALIGN. ii. eapply H in PR. des; eauto.
+    + eapply RANGE. des; eauto.
+Qed.
+
+Lemma private_unfree_inj_wf
+      P j m_src0 m_src1 m_tgt blk_src blk_tgt delta lo hi
+      (INJ: Mem.inject j m_src0 m_tgt)
+      (DELTA: j blk_src = Some (blk_tgt, delta))
+      (PERM: Mem.range_perm m_tgt blk_tgt (delta + lo) (delta + hi) Cur Freeable)
+      (PRVT: range (delta + lo) (delta + hi) <1= loc_out_of_reach j m_src0 blk_tgt)
+      (UNFREE: Mem_unfree m_src0 blk_src lo hi = Some m_src1)
+      (* --------------------------------------------------------- *)
+      (WFINJ: inj_range_wf j m_src0 P)
+      (RANGE: range lo hi <1= P blk_src)
+  :
+    <<WFINJ: inj_range_wf j m_src1 P>>
+.
+Proof.
+  ii. destruct (WFINJ blk).
+  - econs 1; eauto.
+  - econs 2; eauto. ii.
+    eapply ALIGN. ii. eapply H in PR. des; eauto.
+    eapply Mem_unfree_unchanged_on with (P := ~2 brange blk_src lo hi) in UNFREE; eauto.
+    inv UNFREE. specialize (unchanged_on_perm blk x0 k p).
+    destruct (classic (brange blk_src lo hi blk x0)).
+    + right. inv H0. eauto.
+    + left. eapply unchanged_on_perm; eauto.
+      eapply Mem.valid_block_inject_1; eauto.
+Qed.
+
+Lemma private_unfree_inj
+      P j m_src0 m_src1 m_tgt blk_src blk_tgt delta lo hi
+      (INJ: Mem.inject j m_src0 m_tgt)
+      (DELTA: j blk_src = Some (blk_tgt, delta))
+      (PERM: Mem.range_perm m_tgt blk_tgt (delta + lo) (delta + hi) Cur Freeable)
+      (PRVT: range (delta + lo) (delta + hi) <1= loc_out_of_reach j m_src0 blk_tgt)
+      (UNFREE: Mem_unfree m_src0 blk_src lo hi = Some m_src1)
+      (* --------------------------------------------------------- *)
+      (WFINJ: inj_range_wf j m_src0 P)
+      (RANGE: range lo hi <1= P blk_src)
+  :
+    <<INJ: Mem.inject j m_src1 m_tgt>>
+.
+Proof.
+  unfold Mem.inject in *.
+  unfold Mem_unfree in *. des_ifs.
+  inv INJ.
+  econs; eauto.
+  -
+    (* clear_until mi_inj. *)
+
+    inv mi_inj. econs; ii; ss; eauto.
+    + unfold Mem.perm, Mem.perm_order' in H0. ss. des_ifs_safe.
+      rewrite PMap.gsspec in *.
+      destruct (peq b1 blk_src && zle lo ofs && zlt ofs hi) eqn:T; clarify; cycle 1.
+      * eapply mi_perm; eauto. unfold Mem.perm. bsimpl.
+        assert(((Mem.mem_access m_src0) # b1) ofs k = Some p1).
+        { des_ifs; simp. }
+        rewrite H1; ss.
+      * des_ifs; simp.
+        eapply Mem.perm_cur. eapply Mem.perm_implies with Freeable; eauto with mem.
+        eapply PERM; eauto with xomega.
+    + destruct (WFINJ b1); clarify.
+      destruct (eq_block b1 blk_src); clarify.
+      { eapply ALIGN.
+        instantiate (1:=p0). instantiate (1:=Max). instantiate (1:=ofs). ii.
+        unfold Mem.range_perm, Mem.perm in *. ss.
+        rewrite PMap.gss in H0; eauto.
+        specialize (H0 _ PR). unfold proj_sumbool in *. des_ifs; ss; eauto. }
+      * assert (Mem.range_perm m_src0 b1 ofs (ofs + size_chunk chunk) Max p0).
+        { unfold Mem.range_perm, Mem.perm in *. ss.
+          i. specialize (H0 ofs0 H).
+          rewrite PMap.gso in H0; eauto. } clear H0.
+        eapply mi_align; eauto.
+    + unfold Mem.range_perm, Mem.perm in H0; ss.
+      destruct (peq b1 blk_src && zle lo ofs && zlt ofs hi) eqn:T; clarify; cycle 1.
+      * assert(Mem.perm m_src0 b1 ofs Cur Readable).
+        { rewrite PMap.gsspec in H0. des_ifs; simp. }
+        clear H0.
+        rewrite PMap.gsspec.
+        des_ifs; ss; cycle 1.
+        { eapply mi_memval; eauto. }
+        destruct (classic (0 <= hi - lo)); cycle 1.
+        { assert(NEG: exists n, hi - lo = Z.neg n).
+          { assert(Z.sgn (hi - lo) = - 1).
+            { eapply Z.sgn_neg. xomega. }
+            unfold Z.sgn in *. des_ifs. eauto.
+          }
+          des. rewrite NEG. rewrite Z2Nat.inj_neg. ss.
+          eapply mi_memval; eauto.
+        }
+        rewrite Mem.setN_other; ss.
+        { eapply mi_memval; eauto. }
+        ii. rewrite length_list_repeat in *.
+        simp.
+        { rewrite Z2Nat.id in *; ss. xomega. }
+      * simp. rewrite PMap.gsspec. des_ifs.
+        destruct (classic (0 <= hi - lo)); cycle 1.
+        { rewrite PMap.gsspec in *. des_ifs; simp. xomega. }
+        rewrite Mem_setN_in_repeat; ss.
+        { econs; eauto. }
+        rewrite Z2Nat.id; ss.
+        xomega.
+  - clear_until mi_no_overlap.
+    rr. unfold Mem.perm; ss. ii.
+    destruct (peq b1 blk_src && zle lo ofs1 && zlt ofs1 hi) eqn:T1; clarify.
+    { simp. clear mi_no_overlap.
+      rewrite PMap.gss in *. des_ifs; simp. clear H2.
+      rewrite PMap.gso in *; cycle 1.
+      { ii; clarify. }
+      eapply not_and_or. ii. des. clarify.
+      eapply PRVT; try apply H1; eauto; cycle 1.
+      { instantiate (1:= ofs2 + delta2). zsimpl. eauto. }
+      { rr. xomega. }
+    }
+    destruct (peq b2 blk_src && zle lo ofs2 && zlt ofs2 hi) eqn:T2; clarify.
+    { sguard in T1. simp. clear mi_no_overlap.
+      rewrite PMap.gss in *. des_ifs; simp. clear H3.
+      rewrite PMap.gso in *; cycle 1.
+      { ii; clarify. }
+      eapply not_and_or. ii. des. clarify.
+      eapply PRVT; try apply H0; eauto; cycle 1.
+      { instantiate (1:= ofs1 + delta1). zsimpl. eauto. }
+      { rr. xomega. }
+    }
+    specialize (mi_no_overlap b1 b1' delta1 b2 b2' delta2 ofs1 ofs2).
+    do 3 (hexploit1 mi_no_overlap; ss).
+    eapply mi_no_overlap.
+    + rewrite PMap.gsspec in H2. des_ifs; simp.
+    + rewrite PMap.gsspec in H3. des_ifs; simp.
+  - i. ss. destruct (WFINJ b); clarify.
+   destruct (eq_block b blk_src). subst.
+    + des; unfold Mem.perm in *; ss; rewrite PMap.gss in H0.
+      * unfold proj_sumbool in *; des_ifs; eauto 6.
+      * unfold proj_sumbool in *; des_ifs; eauto 6.
+    + assert (Mem.perm m_src0 b (Ptrofs.unsigned ofs) Max Nonempty \/
+              Mem.perm m_src0 b (Ptrofs.unsigned ofs - 1) Max Nonempty).
+      { unfold Mem.range_perm, Mem.perm in *. ss.
+        rewrite PMap.gso in H0; eauto. } clear H0.
+      eapply mi_representable; eauto.
+  - unfold Mem.perm. ss.
+    ii.
+    exploit mi_perm_inv; eauto. i.
+    destruct (peq b1 blk_src && zle lo ofs && zlt ofs hi) eqn:T; clarify.
+    + bsimpl. des_safe. des_sumbool. rewrite PMap.gsspec. des_ifs_safe. ss. left. eauto with mem.
+    + rewrite PMap.gsspec. des_ifs_safe. left. ss. eauto with mem.
+Qed.
 
 Lemma separated_out_of_reach j0 j1 m_src0 m_src1 m_tgt0 blk delta
       (INJ: Mem.inject j0 m_src0 m_tgt0)
@@ -55,78 +235,78 @@ Proof.
   unfold Mem_unfree in *. des_ifs.
 Qed.
 
-Lemma private_unfree_inj j m_src0 m_src1 m_tgt blk_src blk_tgt delta lo hi
-      (DELTA: j blk_src = Some (blk_tgt, delta))
-      (PERM: Mem.range_perm m_tgt blk_tgt (lo+delta) (hi+delta) Cur Freeable) 
-      (PRVT: forall delta' (BOUND: delta + lo <= delta' <delta + hi),
-          loc_out_of_reach j m_src0 blk_tgt delta')
-      (UNFREE: Mem_unfree m_src0 blk_src lo hi = Some m_src1)
-      (INJ: Mem.inject j m_src0 m_tgt)
-  :
-    Mem.inject j m_src1 m_tgt.
-Proof. 
-(*   econs; i. *)
-(*   assert (UNCHANGED: Mem.unchanged_on (~2 brange blk_src lo hi) m_src0 m_src1). *)
-(*   { eapply Mem_unfree_unchanged_on; eauto. } *)
-(*   - econs; i. *)
-(*     destruct (classic (brange blk_src lo hi b1 ofs)); unfold brange in *; ss; *)
-(*       des; clarify. *)
-(*     + eapply Mem.perm_implies. eapply Mem.perm_cur. eapply PERM. *)
-(*       omega. econs. *)
-(*     + eapply Mem.mi_perm;[eapply INJ|..]; eauto. *)
-(*       exploit Mem.unchanged_on_perm; eauto. *)
-(*       instantiate (1 := ofs). instantiate (1 := b1). *)
-(*       unfold brange. ss. *)
-(*       unfold Mem.valid_block. erewrite unfree_nextblock; eauto. *)
-(*       eapply Mem.perm_valid_block; eauto. *)
-(*       i. des. eauto. *)
-(*     + *)
-(*  eapply Mem.mi_align;[eapply INJ|..]; eauto.  *)
-(*     destruct (classic (brange blk_src lo hi b1 (ofs+size_chunk chunk))); unfold brange in *; ss; *)
-(*       des; clarify. *)
-(*     * eapply Mem.perm_implies. eapply Mem.perm_cur. eapply PERM. *)
-(*       omega. econs. *)
-(*     * eapply Mem.mi_perm;[eapply INJ|..]; eauto. *)
-(*       exploit Mem.unchanged_on_perm; eauto. *)
-(*       instantiate (1 := ofs). instantiate (1 := b1). *)
-(*       unfold brange. ss. *)
-(*       unfold Mem.valid_block. erewrite unfree_nextblock; eauto. *)
-(*       eapply Mem.perm_valid_block; eauto. *)
-(*       i. des. eauto. *)
-(* admit "". *)
-(*     + admit "". *)
-(*   - admit "". *)
-(*   - admit "". *)
-(*   - admit "". *)
-(*   - admit "". *)
-(*   - admit "". *)
-(* destruct (eq_block b1 blk_src). *)
-(*     + clarify. destruct (classic (lo <= ofs < hi)). *)
-(*       * eapply Mem.perm_implies. eapply Mem.perm_cur. eapply PERM. *)
-(*         omega. econs. *)
-(*       * eapply Mem.mi_perm;[eapply INJ|..]; eauto. *)
-(*         exploit Mem.unchanged_on_perm; eauto. *)
-(*         instantiate (1 := ofs). instantiate (1 := blk_src). *)
-(*         unfold brange. ss. tauto. *)
-(*         unfold Mem.valid_block. erewrite unfree_nextblock; eauto. *)
-(*         eapply Mem.perm_valid_block; eauto. *)
-(*         i. des. eauto. *)
-(*     + eapply Mem.mi_perm;[eapply INJ|..]; eauto. *)
-(*       exploit Mem.unchanged_on_perm; eauto. *)
-(*       instantiate (1 := ofs). instantiate (1 := b1). *)
-(*       unfold brange. ss. tauto. *)
-(*       unfold Mem.valid_block. erewrite unfree_nextblock; eauto. *)
-(*       eapply Mem.perm_valid_block; eauto. *)
-(*       i. des. eauto. *)
-(*     + eapply Mem.mi_align;[eapply INJ|..]; eauto. admit "". *)
-(*     + admit "". *)
-(*   - admit "". *)
-(*   - admit "". *)
-(*   - admit "". *)
-(*   - admit "". *)
-(*   - admit "". *)
-(*     admit "". *)
-Admitted.
+(* Lemma private_unfree_inj j m_src0 m_src1 m_tgt blk_src blk_tgt delta lo hi *)
+(*       (DELTA: j blk_src = Some (blk_tgt, delta)) *)
+(*       (PERM: Mem.range_perm m_tgt blk_tgt (lo+delta) (hi+delta) Cur Freeable)  *)
+(*       (PRVT: forall delta' (BOUND: delta + lo <= delta' <delta + hi), *)
+(*           loc_out_of_reach j m_src0 blk_tgt delta') *)
+(*       (UNFREE: Mem_unfree m_src0 blk_src lo hi = Some m_src1) *)
+(*       (INJ: Mem.inject j m_src0 m_tgt) *)
+(*   : *)
+(*     Mem.inject j m_src1 m_tgt. *)
+(* Proof.  *)
+(* (*   econs; i. *) *)
+(* (*   assert (UNCHANGED: Mem.unchanged_on (~2 brange blk_src lo hi) m_src0 m_src1). *) *)
+(* (*   { eapply Mem_unfree_unchanged_on; eauto. } *) *)
+(* (*   - econs; i. *) *)
+(* (*     destruct (classic (brange blk_src lo hi b1 ofs)); unfold brange in *; ss; *) *)
+(* (*       des; clarify. *) *)
+(* (*     + eapply Mem.perm_implies. eapply Mem.perm_cur. eapply PERM. *) *)
+(* (*       omega. econs. *) *)
+(* (*     + eapply Mem.mi_perm;[eapply INJ|..]; eauto. *) *)
+(* (*       exploit Mem.unchanged_on_perm; eauto. *) *)
+(* (*       instantiate (1 := ofs). instantiate (1 := b1). *) *)
+(* (*       unfold brange. ss. *) *)
+(* (*       unfold Mem.valid_block. erewrite unfree_nextblock; eauto. *) *)
+(* (*       eapply Mem.perm_valid_block; eauto. *) *)
+(* (*       i. des. eauto. *) *)
+(* (*     + *) *)
+(* (*  eapply Mem.mi_align;[eapply INJ|..]; eauto.  *) *)
+(* (*     destruct (classic (brange blk_src lo hi b1 (ofs+size_chunk chunk))); unfold brange in *; ss; *) *)
+(* (*       des; clarify. *) *)
+(* (*     * eapply Mem.perm_implies. eapply Mem.perm_cur. eapply PERM. *) *)
+(* (*       omega. econs. *) *)
+(* (*     * eapply Mem.mi_perm;[eapply INJ|..]; eauto. *) *)
+(* (*       exploit Mem.unchanged_on_perm; eauto. *) *)
+(* (*       instantiate (1 := ofs). instantiate (1 := b1). *) *)
+(* (*       unfold brange. ss. *) *)
+(* (*       unfold Mem.valid_block. erewrite unfree_nextblock; eauto. *) *)
+(* (*       eapply Mem.perm_valid_block; eauto. *) *)
+(* (*       i. des. eauto. *) *)
+(* (* admit "". *) *)
+(* (*     + admit "". *) *)
+(* (*   - admit "". *) *)
+(* (*   - admit "". *) *)
+(* (*   - admit "". *) *)
+(* (*   - admit "". *) *)
+(* (*   - admit "". *) *)
+(* (* destruct (eq_block b1 blk_src). *) *)
+(* (*     + clarify. destruct (classic (lo <= ofs < hi)). *) *)
+(* (*       * eapply Mem.perm_implies. eapply Mem.perm_cur. eapply PERM. *) *)
+(* (*         omega. econs. *) *)
+(* (*       * eapply Mem.mi_perm;[eapply INJ|..]; eauto. *) *)
+(* (*         exploit Mem.unchanged_on_perm; eauto. *) *)
+(* (*         instantiate (1 := ofs). instantiate (1 := blk_src). *) *)
+(* (*         unfold brange. ss. tauto. *) *)
+(* (*         unfold Mem.valid_block. erewrite unfree_nextblock; eauto. *) *)
+(* (*         eapply Mem.perm_valid_block; eauto. *) *)
+(* (*         i. des. eauto. *) *)
+(* (*     + eapply Mem.mi_perm;[eapply INJ|..]; eauto. *) *)
+(* (*       exploit Mem.unchanged_on_perm; eauto. *) *)
+(* (*       instantiate (1 := ofs). instantiate (1 := b1). *) *)
+(* (*       unfold brange. ss. tauto. *) *)
+(* (*       unfold Mem.valid_block. erewrite unfree_nextblock; eauto. *) *)
+(* (*       eapply Mem.perm_valid_block; eauto. *) *)
+(* (*       i. des. eauto. *) *)
+(* (*     + eapply Mem.mi_align;[eapply INJ|..]; eauto. admit "". *) *)
+(* (*     + admit "". *) *)
+(* (*   - admit "". *) *)
+(* (*   - admit "". *) *)
+(* (*   - admit "". *) *)
+(* (*   - admit "". *) *)
+(* (*   - admit "". *) *)
+(* (*     admit "". *) *)
+(* Admitted. *)
 
 Record freed_from m0 m1 blk lo hi : Prop :=
   mk_freed_from
@@ -209,11 +389,11 @@ Lemma freed_from_out_of_reach j m_src0 m_src1 m_tgt blk lo hi blk' delta ofs
 Proof.
   ii. destruct (eq_block b0 blk).
   - clarify. eapply freed_from_noperm; eauto. omega.
-  - exploit Mem.inject_no_overlap; eauto. 
+  - exploit Mem.inject_no_overlap; eauto.
     + eapply freed_from_perm_le; eauto.
     + eapply Mem.perm_cur.
       eapply Mem.perm_implies.
-      eapply freed_from_perm; eauto. 
+      eapply freed_from_perm; eauto.
       instantiate (1 := ofs - delta). omega. econs.
     + i. des; eauto. omega.
 Qed.
@@ -223,7 +403,21 @@ Definition callee_injection (j: meminj) old_blk new_blk: meminj :=
              then j old_blk
              else (j blk).
 
-Local Ltac simp := repeat (bsimpl; des; des_sumbool; ss; clarify).
+Lemma freed_from_perm_greater m0 m1 blk lo hi
+      (FREE: freed_from m0 m1 blk lo hi)
+  :
+    Mem.perm m1 <4= Mem.perm m0.
+Proof.
+  ii. inv FREE. inv freed_from_unchanged0.
+  specialize (unchanged_on_perm x0 x1 x2 x3).
+  des_ifs; [destruct (zle lo x1); destruct (zlt x1 hi)|];
+    [exploit freed_from_perm0; eauto;
+     i; eapply Mem.perm_cur;
+     eapply Mem.perm_implies; eauto; econs | ..];
+    eapply unchanged_on_perm; eauto with lia;
+      eapply Mem.perm_valid_block in PR; ii;
+        unfold Mem.valid_block; rewrite <- freed_from_nextblock0; auto.
+Qed.
 
 Local Transparent Mem.alloc.
 Lemma memcpy_inject
@@ -291,7 +485,20 @@ Proof.
       * ii; ss. des_ifs.
       * apply NNPP. ii. exploit Mem.mi_freeblocks; eauto. i; clarify.
     + ii; ss.
-      admit "this does not hold".
+      dup FREE. inv FREE. inv freed_from_unchanged0.
+      des_ifs.
+      * eapply mi_align. eauto. instantiate (2 := ofs). ii.
+        assert (Mem.range_perm m_src2 blk_new ofs (ofs+size_chunk chunk) Max p); eauto.
+        assert (range ofs (ofs + size_chunk chunk) <1= range lo hi).
+        { ii. ii. eapply H2 in PR.
+          eapply Mem.perm_alloc_3 in PR; eauto. }
+        apply H3 in H1. eapply freed_from_perm0 in H1.
+        eapply Mem.perm_cur_max. eauto.
+      * eapply mi_align. eauto. instantiate (2 := ofs).
+        eassert (Mem.range_perm m_src2 b1 ofs (ofs+size_chunk chunk) Max p); eauto.
+        eassert (Mem.range_perm m_src1 b1 ofs (ofs+size_chunk chunk) Max p); eauto.
+        { ii. eapply Mem.perm_alloc_4; eauto. }
+        ii. eapply freed_from_perm_greater; eauto.
     + ii; ss. rewrite PMap.gsspec. des_ifs.
       { specialize (mi_memval _ ofs _ _ H).
         unfold Mem.perm in *. ss.
@@ -382,8 +589,23 @@ Proof.
     + assert(Mem.perm m_src1 b2 ofs2 Max Nonempty).
       { eapply Mem.perm_alloc_4; eauto. }
       eapply freed_from_perm_le; eauto.
-  - unfold Mem.perm. ss.
-    admit "this does not hold".
+  - ii. ss. dup FREE. inv FREE. inv freed_from_unchanged0.
+    assert (Mem.perm m_src2 b (Ptrofs.unsigned ofs) Max Nonempty \/
+            Mem.perm m_src2 b (Ptrofs.unsigned ofs - 1) Max Nonempty).
+    { eauto. } clear H0. des_ifs.
+    + eapply mi_representable; eauto.
+      des.
+      * left. exploit freed_from_perm0.
+        { eapply Mem.perm_alloc_3; eauto. }
+        i. eapply Mem.perm_cur_max. eapply Mem.perm_implies; eauto. econs.
+      * right. exploit freed_from_perm0.
+        { eapply Mem.perm_alloc_3; eauto. }
+        i. eapply Mem.perm_cur_max. eapply Mem.perm_implies; eauto. econs.
+    + eapply mi_representable; eauto.
+      assert (Mem.perm m_src1 b (Ptrofs.unsigned ofs) Max Nonempty \/
+              Mem.perm m_src1 b (Ptrofs.unsigned ofs - 1) Max Nonempty).
+      { des; eapply Mem.perm_alloc_4 in H1; eauto. } clear H1.
+      des; [left|right]; eapply freed_from_perm_greater; eauto.
   - unfold Mem.perm. ss.
     ii. des_ifs.
     + destruct (classic (lo <= ofs < hi)).
@@ -449,7 +671,7 @@ Lemma inj_same_inj j v_caller v_callee v_tgt
   :
     Val.inject j v_callee v_tgt.
 Proof.
-  inv SAME. inv INJ. clarify. econs; eauto. 
+  inv SAME. inv INJ. clarify. econs; eauto.
 Qed.
 
 Lemma inj_same_inj2 j v_caller v_callee v_tgt
@@ -458,7 +680,7 @@ Lemma inj_same_inj2 j v_caller v_callee v_tgt
   :
     Val.inject j v_caller v_tgt.
 Proof.
-  inv SAME. inv INJ. clarify. econs; eauto. 
+  inv SAME. inv INJ. clarify. econs; eauto.
 Qed.
 
 Definition to_fake (v: val) : val :=
@@ -479,22 +701,73 @@ Lemma to_fake_inj2 j v_src v_tgt
     Val.inject j v_src v_tgt.
 Proof. unfold to_fake in *. des_ifs; inv INJ; clarify. econs; eauto. Qed.
 
-Lemma unfree_free_inj j (m_src0 m_src1 m_src2 m_tgt: mem) blk0 blk1 delta1 delta2 ofs1 ofs2 size
+Lemma unfree_free_inj P j (m_src0 m_src1 m_src2 m_tgt: mem)
+      blk0 blk1 delta1 delta2 ofs1 ofs2 size
       (DELTA1: delta1 = Ptrofs.unsigned ofs1)
       (DELTA2: delta2 = Ptrofs.unsigned ofs2)
       (FREE: Mem.free m_src0 blk0 delta1 (delta1 + size) = Some m_src1)
       (UNFREE: Mem_unfree m_src1 blk1 delta2 (delta2 + size) = Some m_src2)
       (SAME: inj_same j (Vptr blk1 ofs2 true) (Vptr blk0 ofs1 true))
       (INJ: Mem.inject j m_src0 m_tgt)
+      (WFINJ: inj_range_wf j m_src0 P)
+      (RANGE: range delta2 (delta2 + size) <1= P blk1)
+      (* (WFINJ: inj_range_wf j m_src0 blk1 delta2 (delta2 + size)) *)
   :
     Mem.inject j m_src2 m_tgt.
 Proof.
-  inv SAME. clarify. des_ifs.
-  eapply private_unfree_inj; cycle 3; eauto.
+  inv SAME. clarify. des_ifs. eapply private_unfree_inj; cycle 4; eauto.
+  - ii. destruct (WFINJ blk0).
+    + econs 1; eauto.
+    + econs 2; eauto.
+      i. eapply ALIGN. ii. eapply H in PR. des; eauto.
+      left. eapply Mem.perm_free_3; eauto.
   - eapply Mem.free_left_inject; eauto.
-  - eapply Mem.range_perm_inj; try apply INJ; eauto.
-    eapply Mem.free_range_perm. rewrite Ptrofs.unsigned_zero in *. eauto.
-  - i. intros blk' ofs' INJECT. destruct (eq_block blk' blk_callee); clarify.
+  - rewrite Z.add_comm.
+    replace (delta + (Ptrofs.unsigned Ptrofs.zero + size)) with ((Ptrofs.unsigned Ptrofs.zero + size)+delta) by lia.
+    eapply Mem.range_perm_inj; try apply INJ; eauto.
+    eapply Mem.free_range_perm; eauto.
+  - intros delta' RANGE0 blk' ofs' INJECT. unfold range in *.
+    destruct (eq_block blk' blk_callee); clarify.
+    + eapply Mem.perm_free_2; eauto. lia.
+    + intros PERM. eapply Mem.perm_free_3 in PERM; eauto.
+      eapply Mem.free_range_perm in FREE.
+      exploit Mem.inject_no_overlap; eauto.
+      eapply Mem.perm_max; eauto.
+      eapply Mem.perm_implies; eauto.
+      eapply FREE; eauto.
+      * assert (Ptrofs.unsigned Ptrofs.zero <= delta' - delta < Ptrofs.unsigned Ptrofs.zero + size).
+        rewrite Ptrofs.unsigned_zero in *. lia. eauto.
+      * econs.
+      * splits. des; eauto. lia.
+Qed.
+
+Lemma unfree_free_inj_wf P j (m_src0 m_src1 m_src2 m_tgt: mem)
+      blk0 blk1 delta1 delta2 ofs1 ofs2 size
+      (DELTA1: delta1 = Ptrofs.unsigned ofs1)
+      (DELTA2: delta2 = Ptrofs.unsigned ofs2)
+      (FREE: Mem.free m_src0 blk0 delta1 (delta1 + size) = Some m_src1)
+      (UNFREE: Mem_unfree m_src1 blk1 delta2 (delta2 + size) = Some m_src2)
+      (SAME: inj_same j (Vptr blk1 ofs2 true) (Vptr blk0 ofs1 true))
+      (INJ: Mem.inject j m_src0 m_tgt)
+      (WFINJ: inj_range_wf j m_src0 P)
+      (RANGE: range delta2 (delta2 + size) <1= P blk1)
+      (* (WFINJ: inj_range_wf j m_src0 blk1 delta2 (delta2 + size)) *)
+  :
+    inj_range_wf j m_src2 P.
+Proof.
+  inv SAME. clarify. des_ifs. eapply private_unfree_inj_wf; cycle 4; eauto.
+  - ii. destruct (WFINJ blk0).
+    + econs 1; eauto.
+    + econs 2; eauto.
+      i. eapply ALIGN. ii. eapply H in PR. des; eauto.
+      left. eapply Mem.perm_free_3; eauto.
+  - eapply Mem.free_left_inject; eauto.
+  - rewrite Z.add_comm.
+    replace (delta + (Ptrofs.unsigned Ptrofs.zero + size)) with ((Ptrofs.unsigned Ptrofs.zero + size)+delta) by lia.
+    eapply Mem.range_perm_inj; try apply INJ; eauto.
+    eapply Mem.free_range_perm; eauto.
+  - intros delta' RANGE0 blk' ofs' INJECT. unfold range in *.
+    destruct (eq_block blk' blk_callee); clarify.
     + eapply Mem.perm_free_2; eauto. lia.
     + intros PERM. eapply Mem.perm_free_3 in PERM; eauto.
       eapply Mem.free_range_perm in FREE.
@@ -514,7 +787,7 @@ Lemma memcpy_load
       (FREE: freed_from m_src0 m_src1 blk_old lo hi)
       (ALLOC: Mem.alloc m_src1 lo hi = (m_src2, blk_new))
       (BOUND0: lo <= ofs)
-      (BOUND1: ofs + size_chunk chunk <= hi) 
+      (BOUND1: ofs + size_chunk chunk <= hi)
       (LOAD: Mem.load chunk m_src0 blk_old ofs = Some v)
   :
     Mem.load chunk (memcpy m_src2 blk_old blk_new)
